lib_list/Test.LList.fst
@@ -10,23 +10,26 @@ module U64 = FStar.UInt64
 
 open Selectors.LList
 
+[@@__reduce__]
+unfold let p = fun _ -> emp
+
 let temp (_:unit)
   : Steel (t U64.t)
   emp
-  (fun ptr -> llist (fun _ -> emp) ptr)
+  (fun ptr -> llist p ptr)
   (requires fun _ -> True)
   (ensures fun _ ptr h1 ->
-    v_llist (fun _ -> emp) ptr h1 == [ 1UL ; 0UL ]
+    v_llist p ptr h1 == [ 1UL ; 0UL ]
   )
   =
   let c1 = mk_cell null_t 0UL in
   let r1 = malloc c1 in
   let c2 = mk_cell r1 1UL in
   let r2 = malloc c2 in
-  intro_llist_nil (fun _ -> emp);
-  pack_list (fun _ -> emp) r1 null_t 0UL;
-  pack_list (fun _ -> emp) r2 r1 1UL;
-  cons_is_not_null (fun _ -> emp) r2;
-  let n = unpack_list (fun _ -> emp) r2 in
-  pack_list (fun _ -> emp) r2 (get_next n) 1UL;
+  intro_llist_nil p;
+  pack_list p r1 null_t 0UL;
+  pack_list p r2 r1 1UL;
+  cons_is_not_null p r2;
+  let n = unpack_list p r2 in
+  pack_list p r2 (get_next n) 1UL;
   return r2
